extraction/theories/MidlangExtract.v
@@ -572,7 +572,6 @@ Definition print_mutual_inductive_body
                  name <- fresh_ty_arg_name (tvar_name name) Γ;;
                  ret (Γ ++ [name])%list) (ind_ctor_type_vars oib) [];;
 
-
        (fix print_ind_ctors (ctors : list (ident * list box_type)) prefix :=
           match ctors with
           | [] => ret tt
